example/ttcan/Network.TTCan.Extract.fst
@@ -1,6 +1,7 @@
 module Network.TTCan.Extract
 
-module Top = Network.TTCan.CycleTime
+module Types = Network.TTCan.Types
+module Top = Network.TTCan.Impl.States
 
 module SugarBase = Pipit.Sugar.Base
 module XX  = Pipit.Exec.Exp
@@ -15,12 +16,12 @@ let expr = SugarBase.exp_of_stream2 Top.top
 [@@(Tac.postprocess_with (XL.tac_normalize_pure ["Network.TTCan"]))]
 type state = XX.state_of_exp expr
 
-type result = Top.ntu
+type result = Types.ntu
 
 [@@(Tac.postprocess_with (XL.tac_normalize_pure ["Network.TTCan"]))]
 noextract
 inline_for_extraction
-let system: XX.esystem (Top.ntu & (bool & unit)) state result =
+let system: XX.esystem (Types.ntu & (bool & unit)) state result =
   assert_norm (XX.extractable expr);
   XX.exec_of_exp expr
 
@@ -28,4 +29,4 @@ let system: XX.esystem (Top.ntu & (bool & unit)) state result =
 let reset = XL.mk_reset system
 
 [@@(Tac.postprocess_with (XL.tac_extract ["Network.TTCan"]))]
-let step (local_time: Top.ntu) (reset_ck: bool) = XL.mk_step system (local_time, (reset_ck, ()))
+let step (local_time: Types.ntu) (reset_ck: bool) = XL.mk_step system (local_time, (reset_ck, ()))
