example/ttcan/Network.TTCan.Impl.States.fst
@@ -1,0 +1,226 @@
+module Network.TTCan.Impl.States
+
+module S       = Pipit.Sugar.Shallow
+module Clocked = Network.TTCan.Prim.Clocked
+module S32R    = Network.TTCan.Prim.S32R
+module U64     = Network.TTCan.Prim.U64
+
+module Util = Network.TTCan.Impl.Util
+
+open Network.TTCan.Types
+
+let cycle_time_capture
+  (local_time: S.stream ntu)
+  (reset_ck:           S.stream bool)
+  (cycle_time_capture: S.stream (Clocked.t ntu))
+    : S.stream ntu =
+  let open S in
+  let open U64 in
+  let^ cycle_time_start = rec' (fun cycle_time_start ->
+    let dflt = if_then_else reset_ck
+      local_time
+      (0uL `fby` cycle_time_start) in
+    Clocked.get_or_else dflt cycle_time_capture) in
+  let^ cycle_time = local_time - cycle_time_start in
+  // check "" (sofar (time_ascending local_time /\ cycle_time_capture <= local_time) ==> cycle_time <= local_time);^
+  cycle_time
+
+let mode_states
+  (mode_cmd: S.stream (Clocked.t mode))
+    : S.stream mode =
+  let open S in
+  rec' (fun mode ->
+    Clocked.get_or_else
+      (Mode_Configure `fby` mode)
+      mode_cmd)
+
+let sync_states
+  (mode:       S.stream mode)
+  (error:      S.stream error_severity)
+  (ref_mark:   S.stream (Clocked.t ntu))
+  (local_time: S.stream ntu)
+    : S.stream (sync_mode & ntu) =
+  let open S in
+  // Reset cycle_time=0 when leaving configure to satisfy Sync_Mode.TS1 below; also reset when in configure time to avoid returning an invalid cycle time
+  let^ cycle_time_reset = (mode = const Mode_Configure \/ pre (mode = const Mode_Configure)) in
+  let^ cycle_time = cycle_time_capture local_time cycle_time_reset ref_mark in
+  (*^9.4.2 transition Sync_Mode.TS1: Config_Mode is left, Cycle_Time shall be zero *)
+  // --%PROPERTY "^9.4.2 Sync_Mode.TS1: Config_Mode is left, Cycle_Time shall be zero" falling_edge(mode = Mode_Configure) => cycle_time = 0;
+  // --%PROPERTY "Sync_Mode.Cycle_Time:ref_mark reset" sync_state = In_Schedule and ref_mark_ck => cycle_time = local_time - ref_mark;
+
+  (*^9.4.2 Sync_Mode *)
+  let sync_state = rec' (fun sync_state ->
+    let^ pre_sync = Sync_Off `fby` sync_state in
+    let^ seen_sync_ref_mark = Util.latch { set = Clocked.get_clock ref_mark; reset = (pre_sync <> const Synchronising) } in
+
+    (*^9.4.2 transition Sync_Mode.TS0: transition condition always taking prevalance; HW reset or (Mode = Config) or (error state = S3) *)
+    if_then_else (mode = const Mode_Configure \/ error = const S3_Severe)
+      (const Sync_Off)
+      (*^9.4.2 State Sync_Off: No synchronisation activity in progress.. *)
+      (if_then_else (pre_sync = const Sync_Off)
+      (*^9.4.2 transition Sync_Mode.TS1: Config_Mode is left, Cycle_Time shall be zero *)
+        (const Synchronising)
+        (*^9.4.2 State Synchronising: FSE is in process of synchronisation but not yet synchronised. *)
+        (if_then_else (pre_sync = const Synchronising)
+          (*^9.4.2 transition Sync_Mode.TS3: at least two successive reference messages observed (the last reference message did not contain a set Disc_Bit), last reference message did not contain a Next_Is_Gap bit *)
+          //^8.2 After reset, a FSE shall consider itself synchronised to the network after the occurrence of the second consecutive reference message
+          (if_then_else (pre seen_sync_ref_mark /\ Clocked.get_clock ref_mark)
+            (const In_Schedule)
+            (*^9.4.2 NOTIMPLEMENTED Next_Is_Gap: transition Sync_Mode.TS2: at least two successive reference messages observed (the last reference message did not contain a set Disc_Bit), last reference message contained a Next_Is_Gap bit *)
+            (const Synchronising))
+          (if_then_else (pre_sync = const In_Schedule)
+            (*^9.4.2 State In_Schedule: FSE is synchronised, no gap expected. *)
+            (*^9.4.2 NOTIMPLEMENTED Next_Is_Gap: transition Sync_Mode.TS4: Next_Is_Gap = 1 observed in reference message *)
+            (const In_Schedule)
+            // IMPOSSIBLE
+            (const Sync_Off)))))
+  in
+  tup sync_state cycle_time
+  // --%PROPERTY mode = Mode_Configure => sync_state = Sync_Off;
+  // --%PROPERTY error = S3_Severe => sync_state = Sync_Off;
+
+
+let master_modes
+  (cfg:     config)
+  (mode:    S.stream mode)
+  (error:   S.stream error_severity)
+  (ref_msg: S.stream (Clocked.t master_index))
+    : S.stream master_mode =
+  let open S in
+  let^ master_enable = const (config_master_enable cfg) in
+  let^ master_index  = const (config_master_index cfg) in
+
+  rec' (fun master_mode ->
+    let^ pre_master = Master_Off `fby` master_mode in
+
+    // --%PROPERTY "Master_Mode.Master_Off.enabled-on-message" ref_msg_ck and mode <> Mode_Configure and error <> S2_Error and error <> S3_Severe => master_mode <> Master_Off;
+    // --%PROPERTY "Master_Mode.master-not-follower" config_master_enable => master_mode <> Follower;
+    // --%PROPERTY "Master_Mode.follower-not-master" not config_master_enable => master_mode = Master_Off or master_mode = Follower;
+    // --%PROPERTY "Master_Mode.error-S2" error = S2_Error => master_mode = Master_Off or master_mode = Follower;
+
+    (*^9.4.3 transition Master_Mode.TM0: transition condition always taking prevalence; HW reset or (Mode = Config) or (error state = S3) *)
+    // --%PROPERTY "^9.4.3 Master_Mode.TM0.1(reset)" (true -> false) and not ref_msg_ck => master_mode = Master_Off;
+    // --%PROPERTY "^9.4.3 Master_Mode.TM0.2" mode = Mode_Configure or error = S3_Severe => master_mode = Master_Off;
+
+    (*^9.4.3 transition Master_Mode.TM1 (from Master_Off): FSE is not potential master and a reference message is observed *)
+    // --%PROPERTY "^9.4.3 Master_Mode.TM1" mode <> Mode_Configure and No_Error(error) and not config_master_enable and ref_msg_ck => master_mode = Follower;
+
+    (*^9.4.3 transition Master_Mode.TM2 (from Master_Off): FSE is potential master, error state is not S2 or S3, reference message is observed from other master *)
+    (*^9.4.3 transition Master_Mode.TM3 (from Master_Off): FSE is potential master, error state is not S2 or S3, reference message is observed from self *)
+
+    (*^9.4.3 transition Master_Mode.TM4 (from Backup_Master): FSE changes from backup master to current master when it observes a reference message with its own time master priority *)
+    (*^9.4.3 transition Master_Mode.TM6 (from Backup_Master): error state = S2 *)
+
+    (*^9.4.3 transition Master_Mode.TM5 (from Current_Master): FSE changes from current master to backup master when it observes a reference message with a time master priority higher than its own *)
+    (*^9.4.3 transition Master_Mode.TM7 (from Current_Master): error state = S2 *)
+
+    (*^9.4.3 transition Master_Mode.TM0: transition condition always taking prevalence; HW reset or (Mode = Config) or (error state = S3) *)
+    if_then_else (mode = const Mode_Configure \/ error = const S3_Severe)
+      (const Master_Off)
+      (if_then_else (pre_master = const Master_Off)
+        (if_then_else (Clocked.get_clock ref_msg /\ ~ master_enable)
+          (const Follower)
+          (if_then_else (Clocked.get_clock ref_msg /\ master_enable /\ error <> const S2_Error)
+            (if_then_else (Clocked.get_value ref_msg = master_index)
+              (const Current_Master)
+              (const Backup_Master))
+            (const Master_Off))
+        )
+        (if_then_else (pre_master = const Backup_Master)
+          (if_then_else (error = const S2_Error)
+            (const Master_Off)
+            (if_then_else S32R.(Clocked.get_clock ref_msg /\ Clocked.get_value ref_msg < master_index)
+              (const Backup_Master)
+              (const Current_Master)))
+          (if_then_else (pre_master = const Follower)
+            (const Follower)
+            // impossible
+            (const Master_Off)))))
+
+let ref_trigger_offsets
+  (cfg:         config)
+  (master_mode: S.stream master_mode)
+  (error:       S.stream error_severity)
+  (ref_master:  S.stream (Clocked.t master_index))
+    : S.stream ref_offset =
+  let open S in
+  let open S32R in
+  let^ master_index = const (config_master_index cfg) in
+  rec' (fun ref_trigger_offset ->
+    let^ pre_ref = cfg.initial_ref_offset `fby` ref_trigger_offset in
+    //^ If [a potential master] becomes current time master (by successfully transmitting a reference message), it shall use Ref_Trigger_Offset = 0.
+    if_then_else (master_mode = const Current_Master)
+      (s32r 0)
+      //^ [At error level S2,] potential masters may still transmit reference messages with the Ref_Trigger_Offset set to the maximum value of 127.
+      (if_then_else (error = const S2_Error)
+        (s32r 127)
+        // Downgrading to a backup master
+        (if_then_else (Util.rising_edge (master_mode = const Backup_Master))
+          (const cfg.initial_ref_offset)
+          // If we start a new basic cycle and the current master is higher index (lower priority) than us, we want to try to reduce our ref offset to overtake the current master
+          (if_then_else (Clocked.get_clock ref_master /\ Clocked.get_value ref_master > master_index)
+            (if_then_else (pre_ref > s32r 0)
+              (s32r 0)
+              (dec_sat pre_ref))
+            pre_ref))))
+
+
+let rx_ref_filters
+  (rx_ref:     S.stream (Clocked.t ref_message))
+  (pre_tx_ref: S.stream (Clocked.t ref_message))
+  (pre_tx_status: S.stream tx_status)
+    : S.stream (Clocked.t ref_message) =
+  let open S in
+  let^ tx_success = Clocked.get_clock pre_tx_ref /\ pre_tx_status = const Tx_Ok in
+  let^ last_ref =
+    if_then_else (Clocked.get_clock rx_ref /\ Clocked.get_clock pre_tx_ref)
+      (if_then_else U64.(get_sof (Clocked.get_value rx_ref) <= get_sof (Clocked.get_value pre_tx_ref))
+        rx_ref
+        pre_tx_ref)
+      (if_then_else (Clocked.get_clock rx_ref)
+        rx_ref
+        pre_tx_ref) in
+  last_ref
+
+let tx_ref_messages
+  (cfg:        config)
+  (local_time: S.stream ntu)
+  (sync_state: S.stream sync_mode)
+  (error:      S.stream error_severity)
+  (cycle_time: S.stream ntu)
+  (cycle_index:S.stream cycle_index)
+  (send_ck:    S.stream bool)
+    : S.stream (Clocked.t ref_message) =
+  let open S in
+  let^ severe_error_cooldown = rec' (fun severe_error_cooldown ->
+    if_then_else
+      (error = const S3_Severe)
+      U64.(local_time + S32R.s32r_to_u64 (const cfg.severe_error_ref_cooldown))
+      (0uL `fby` severe_error_cooldown)) in
+
+  let^ cycle_index' = S32R.(
+        if_then_else S32R.(cycle_index < const cfg.cycle_count_max)
+          (inc_sat cycle_index)
+          (s32r 0)) in
+
+  let^ tx_ref =
+    ref_message_new
+      local_time
+      (const (config_master_index cfg))
+      cycle_index' in
+
+  let^ tx_ref_ck =
+    (sync_state = const Synchronising \/ sync_state = const In_Schedule) /\
+    send_ck /\
+    U64.(severe_error_cooldown < local_time) in
+
+  //%PROPERTY "^9.1:severe-no-transmission" error = S3_Severe => not tx_ref_ck;
+
+  if_then_else tx_ref_ck
+    (Clocked.some tx_ref)
+    Clocked.none
+
+
+let top (local_time: S.stream ntu) (reset_ck: S.stream bool): S.stream ntu =
+  cycle_time_capture local_time reset_ck (Clocked.some (S.const 0uL))
+
